Rewriting semantics/proof system rules

formalization/mfotl/thys/Proof_System.thy
@@ -8,57 +8,93 @@ definition ETP:: "'a trace \<Rightarrow> nat \<Rightarrow> nat"  where
 definition LTP:: "'a trace \<Rightarrow> nat \<Rightarrow> nat" where
     "LTP \<sigma> ts = Max {i. (\<tau> \<sigma> i) \<le> ts}"
 
+abbreviation "\<delta> \<sigma> i j \<equiv> (\<tau> \<sigma> i - \<tau> \<sigma> j)"
+
+abbreviation "ETP_p \<sigma> i b \<equiv> ETP \<sigma> ((\<tau> \<sigma> i) - b)"
 abbreviation "LTP_p \<sigma> i I \<equiv> min i (LTP \<sigma> ((\<tau> \<sigma> i) - left I))"
 abbreviation "ETP_f \<sigma> i I \<equiv> max i (ETP \<sigma> ((\<tau> \<sigma> i) + left I))"
+abbreviation "LTP_f \<sigma> i b \<equiv> LTP \<sigma> ((\<tau> \<sigma> i) + b)"
 
-inductive SAT and VIO :: "'a Extended_MFOTL.trace \<Rightarrow> 'a Extended_MFOTL.env \<Rightarrow> nat \<Rightarrow> 'a Extended_MFOTL.formula \<Rightarrow> bool" where
-  SPred: "(r, map (Extended_MFOTL.eval_trm v) trms) \<in> \<Gamma> \<sigma> i \<Longrightarrow> SAT \<sigma> v i (Extended_MFOTL.Pred r trms)"
-| VPred: "(r, map (Extended_MFOTL.eval_trm v) trms) \<notin> \<Gamma> \<sigma> i \<Longrightarrow> VIO \<sigma> v i (Extended_MFOTL.Pred r trms)"
-| SEq: "(Extended_MFOTL.eval_trm v t1) = (Extended_MFOTL.eval_trm v t2) \<Longrightarrow> SAT \<sigma> v i (Extended_MFOTL.Eq t1 t2)"
-| VEq: "(Extended_MFOTL.eval_trm v t1) \<noteq> (Extended_MFOTL.eval_trm v t2) \<Longrightarrow> VIO \<sigma> v i (Extended_MFOTL.Eq t1 t2)"
-| SNeg: "VIO \<sigma> v i \<phi> \<Longrightarrow> SAT \<sigma> v i (Extended_MFOTL.Neg \<phi>)"
-| VNeg: "SAT \<sigma> v i \<phi> \<Longrightarrow> VIO \<sigma> v i (Extended_MFOTL.Neg \<phi>)"
-| SDisjL: "SAT \<sigma> v i \<phi> \<Longrightarrow> SAT \<sigma> v i (Extended_MFOTL.Or \<phi> \<psi>)"
-| SDisjR: "SAT \<sigma> v i \<psi> \<Longrightarrow> SAT \<sigma> v i (Extended_MFOTL.Or \<phi> \<psi>)"
-| VDisj: "VIO \<sigma> v i \<phi> \<Longrightarrow> VIO \<sigma> v i \<psi> \<Longrightarrow> VIO \<sigma> v i (Extended_MFOTL.Or \<phi> \<psi>)"
+inductive SAT and VIO :: "'a MFOTL.trace \<Rightarrow> 'a MFOTL.env \<Rightarrow> nat \<Rightarrow> 'a MFOTL.formula \<Rightarrow> bool" where
+  STT: "SAT \<sigma> v i TT"
+| VFF: "VIO \<sigma> v i FF"
+| SPred: "(r, MFOTL.eval_trms v ts) \<in> \<Gamma> \<sigma> i \<Longrightarrow> SAT \<sigma> v i (MFOTL.Pred r ts)"
+| VPred: "(r, MFOTL.eval_trms v ts) \<notin> \<Gamma> \<sigma> i \<Longrightarrow> VIO \<sigma> v i (MFOTL.Pred r ts)"
+| SEq: "(MFOTL.eval_trm v t1) = (MFOTL.eval_trm v t2) \<Longrightarrow> SAT \<sigma> v i (MFOTL.Eq t1 t2)"
+| VEq: "(MFOTL.eval_trm v t1) \<noteq> (MFOTL.eval_trm v t2) \<Longrightarrow> VIO \<sigma> v i (MFOTL.Eq t1 t2)"
+| SNeg: "VIO \<sigma> v i \<phi> \<Longrightarrow> SAT \<sigma> v i (MFOTL.Neg \<phi>)"
+| VNeg: "SAT \<sigma> v i \<phi> \<Longrightarrow> VIO \<sigma> v i (MFOTL.Neg \<phi>)"
+| SOrL: "SAT \<sigma> v i \<phi> \<Longrightarrow> SAT \<sigma> v i (MFOTL.Or \<phi> \<psi>)"
+| SOrR: "SAT \<sigma> v i \<psi> \<Longrightarrow> SAT \<sigma> v i (MFOTL.Or \<phi> \<psi>)"
+| VOr: "VIO \<sigma> v i \<phi> \<Longrightarrow> VIO \<sigma> v i \<psi> \<Longrightarrow> VIO \<sigma> v i (MFOTL.Or \<phi> \<psi>)"
+| SAnd: "SAT \<sigma> v i \<phi> \<Longrightarrow> SAT \<sigma> v i \<psi> \<Longrightarrow> SAT \<sigma> v i (MFOTL.And \<phi> \<psi>)"
+| VAndL: "VIO \<sigma> v i \<phi> \<Longrightarrow> VIO \<sigma> v i (MFOTL.And \<phi> \<psi>)"
+| VAndR: "VIO \<sigma> v i \<psi> \<Longrightarrow> VIO \<sigma> v i (MFOTL.And \<phi> \<psi>)"
+| SImplL: "VIO \<sigma> v i \<phi> \<Longrightarrow> SAT \<sigma> v i (MFOTL.Imp \<phi> \<psi>)"
+| SImplR: "SAT \<sigma> v i \<psi> \<Longrightarrow> SAT \<sigma> v i (MFOTL.Imp \<phi> \<psi>)"
+| VImpl: "SAT \<sigma> v i \<phi> \<Longrightarrow> VIO \<sigma> v i \<psi> \<Longrightarrow> VIO \<sigma> v i (MFOTL.Imp \<phi> \<psi>)"
+| SIffSS: "SAT \<sigma> v i \<phi> \<Longrightarrow> SAT \<sigma> v i \<psi> \<Longrightarrow> SAT \<sigma> v i (MFOTL.Iff \<phi> \<psi>)"
+| SIffVV: "VIO \<sigma> v i \<phi> \<Longrightarrow> VIO \<sigma> v i \<psi> \<Longrightarrow> SAT \<sigma> v i (MFOTL.Iff \<phi> \<psi>)"
+| VIffSV: "SAT \<sigma> v i \<phi> \<Longrightarrow> VIO \<sigma> v i \<psi> \<Longrightarrow> VIO \<sigma> v i (MFOTL.Iff \<phi> \<psi>)"
+| VIffVS: "VIO \<sigma> v i \<phi> \<Longrightarrow> SAT \<sigma> v i \<psi> \<Longrightarrow> VIO \<sigma> v i (MFOTL.Iff \<phi> \<psi>)"
 
-| SExists: "SAT \<sigma> (x # v) i \<phi> \<Longrightarrow> SAT \<sigma> v i (Extended_MFOTL.Exists \<phi>)"
-| VExists: "VIO \<sigma> (x # v) i \<phi> \<Longrightarrow> VIO \<sigma> v i (Extended_MFOTL.Exists \<phi>)"
+| SExists: "SAT \<sigma> v i \<phi> \<Longrightarrow> SAT \<sigma> v i (MFOTL.Exists \<phi>)"
+| VExists: "VIO \<sigma> v i \<phi> \<Longrightarrow> VIO \<sigma> v i (MFOTL.Exists \<phi>)"
 
-
-| SNext: "mem (\<Delta> \<sigma> (i+1)) I \<Longrightarrow> SAT \<sigma> v (i+1) \<phi> \<Longrightarrow> SAT \<sigma> v i (Extended_MFOTL.Next I \<phi>)"
-| VNext: "VIO \<sigma> v (i+1) \<phi> \<Longrightarrow> VIO \<sigma> v i (Extended_MFOTL.Next I \<phi>)"
-| VNext_le: "(\<Delta> \<sigma> (i+1)) < (left I) \<Longrightarrow> VIO \<sigma> v i (Extended_MFOTL.Next I \<phi>)"
-| VNext_ge: "enat (\<Delta> \<sigma> (i+1)) > (right I) \<Longrightarrow> VIO \<sigma> v i (Extended_MFOTL.Next I \<phi>)"
-| SPrev: "i > 0 \<Longrightarrow> mem (\<Delta> \<sigma> i) I \<Longrightarrow> SAT \<sigma> v (i-1) \<phi> \<Longrightarrow> SAT \<sigma> v i (Extended_MFOTL.Prev I \<phi>)"
-| VPrev: "i > 0 \<Longrightarrow> VIO \<sigma> v (i-1) \<phi> \<Longrightarrow> VIO \<sigma> v i (Extended_MFOTL.Prev I \<phi>)"
-| VPrev_zero: "i = 0 \<Longrightarrow> VIO \<sigma> v i (Extended_MFOTL.Prev I \<phi>)"
-| VPrev_le: "i > 0 \<Longrightarrow> (\<Delta> \<sigma> i) < (left I) \<Longrightarrow> VIO \<sigma> v i (Extended_MFOTL.Prev I \<phi>)"
-| VPrev_ge: "i > 0 \<Longrightarrow> enat (\<Delta> \<sigma> i) > (right I) \<Longrightarrow> VIO \<sigma> v i (Extended_MFOTL.Prev I \<phi>)"
-| SSince: "j \<le> i \<Longrightarrow> mem (\<tau> \<sigma> i - \<tau> \<sigma> j) I  \<Longrightarrow> SAT \<sigma> v j \<psi> \<Longrightarrow> (\<And>k. k \<in> {j <.. i}
-            \<Longrightarrow> SAT \<sigma> v k \<phi>) \<Longrightarrow> SAT \<sigma> v i (Extended_MFOTL.Since \<phi> I \<psi>)"
-| VSince_le: "\<tau> \<sigma> i < \<tau> \<sigma> 0 + left I \<Longrightarrow> VIO \<sigma> v i (Extended_MFOTL.Since \<phi> I \<psi>)"
+| SPrev: "i > 0 \<Longrightarrow> mem (\<Delta> \<sigma> i) I \<Longrightarrow> SAT \<sigma> v (i-1) \<phi> \<Longrightarrow> SAT \<sigma> v i (MFOTL.Prev I \<phi>)"
+| VPrev: "i > 0 \<Longrightarrow> VIO \<sigma> v (i-1) \<phi> \<Longrightarrow> VIO \<sigma> v i (MFOTL.Prev I \<phi>)"
+| VPrevZ: "i = 0 \<Longrightarrow> VIO \<sigma> v i (MFOTL.Prev I \<phi>)"
+| VPrevOutL: "i > 0 \<Longrightarrow> (\<Delta> \<sigma> i) < (left I) \<Longrightarrow> VIO \<sigma> v i (MFOTL.Prev I \<phi>)"
+| VPrevOutR: "i > 0 \<Longrightarrow> enat (\<Delta> \<sigma> i) > (right I) \<Longrightarrow> VIO \<sigma> v i (MFOTL.Prev I \<phi>)"
+| SNext: "mem (\<Delta> \<sigma> (i+1)) I \<Longrightarrow> SAT \<sigma> v (i+1) \<phi> \<Longrightarrow> SAT \<sigma> v i (MFOTL.Next I \<phi>)"
+| VNext: "VIO \<sigma> v (i+1) \<phi> \<Longrightarrow> VIO \<sigma> v i (MFOTL.Next I \<phi>)"
+| VNextOutL: "(\<Delta> \<sigma> (i+1)) < (left I) \<Longrightarrow> VIO \<sigma> v i (MFOTL.Next I \<phi>)"
+| VNextOutR: "enat (\<Delta> \<sigma> (i+1)) > (right I) \<Longrightarrow> VIO \<sigma> v i (MFOTL.Next I \<phi>)"
+| SOnce: "j \<le> i \<Longrightarrow> mem (\<delta> \<sigma> i j) I \<Longrightarrow> SAT \<sigma> v j \<phi> \<Longrightarrow> SAT \<sigma> v i (MFOTL.Once I \<phi>)"
+| VOnceOut: "\<tau> \<sigma> i < \<tau> \<sigma> 0 + left I \<Longrightarrow> VIO \<sigma> v i (MFOTL.Once I \<phi>)"
+| VOnce: "j = (case right I of \<infinity> \<Rightarrow> 0 
+               | enat b \<Rightarrow> ETP_p \<sigma> i b) \<Longrightarrow>
+          (\<tau> \<sigma> i) \<ge> (\<tau> \<sigma> 0) + left I \<Longrightarrow>
+          (\<And>k. k \<in> {j .. LTP_p \<sigma> i I} \<Longrightarrow> VIO \<sigma> v k \<phi>) \<Longrightarrow> VIO \<sigma> v i (MFOTL.Once I \<phi>)"
+| SHist: "j = (case right I of \<infinity> \<Rightarrow> 0 
+               | enat b \<Rightarrow> ETP_p \<sigma> i b) \<Longrightarrow>
+          (\<tau> \<sigma> i) \<ge> (\<tau> \<sigma> 0) + left I \<Longrightarrow>
+          (\<And>k. k \<in> {j .. LTP_p \<sigma> i I} \<Longrightarrow> SAT \<sigma> v k \<phi>) \<Longrightarrow> SAT \<sigma> v i (MFOTL.Hist I \<phi>)"
+| SHistoricallyOut: "\<tau> \<sigma> i < \<tau> \<sigma> 0 + left I \<Longrightarrow> SAT \<sigma> v i (MFOTL.Hist I \<phi>)"
+| VHistorically: "j \<le> i \<Longrightarrow> mem (\<delta> \<sigma> i j) I  \<Longrightarrow> VIO \<sigma> v j \<phi> \<Longrightarrow> VIO \<sigma> v i (MFOTL.Hist I \<phi>)"
+| SEventually: "j \<ge> i \<Longrightarrow> mem (\<delta> \<sigma> j i) I  \<Longrightarrow> SAT \<sigma> v j \<phi> \<Longrightarrow> SAT \<sigma> v i (MFOTL.Event I \<phi>)"
+| VEventually: "(\<And>k. k \<in> (case right I of \<infinity> \<Rightarrow> {ETP_f \<sigma> i I ..}
+                           | enat b \<Rightarrow> {ETP_f \<sigma> i I .. LTP_f \<sigma> i b}) \<Longrightarrow> VIO \<sigma> v k \<phi>) \<Longrightarrow> 
+                VIO \<sigma> v i (MFOTL.Event I \<phi>)"
+| SAlways: "(\<And>k. k \<in> (case right I of \<infinity> \<Rightarrow> {lu i I ..} 
+                       | enat b \<Rightarrow> {ETP_f \<sigma> i I .. LTP_f \<sigma> i b}) \<Longrightarrow> SAT \<sigma> v k \<phi>) \<Longrightarrow>
+            SAT \<sigma> v i (MFOTL.Always I \<phi>)"
+| VAlways: "j \<ge> i \<Longrightarrow> mem (\<delta> \<sigma> j i) I  \<Longrightarrow> VIO \<sigma> v j \<phi> \<Longrightarrow> VIO \<sigma> v i (MFOTL.Always I \<phi>)"
+| SSince: "j \<le> i \<Longrightarrow> mem (\<delta> \<sigma> i j) I  \<Longrightarrow> SAT \<sigma> v j \<psi> \<Longrightarrow> (\<And>k. k \<in> {j <.. i} \<Longrightarrow> 
+           SAT \<sigma> v k \<phi>) \<Longrightarrow> SAT \<sigma> v i (MFOTL.Since \<phi> I \<psi>)"
+| VSinceOut: "\<tau> \<sigma> i < \<tau> \<sigma> 0 + left I \<Longrightarrow> VIO \<sigma> v i (MFOTL.Since \<phi> I \<psi>)"
 | VSince: "(case right I of \<infinity> \<Rightarrow> True 
             | enat b \<Rightarrow> ETP \<sigma> ((\<tau> \<sigma> i) - b) \<le> j) \<Longrightarrow> 
-            j \<le> i \<Longrightarrow> (\<tau> \<sigma> 0) + left I \<le> (\<tau> \<sigma> i) \<Longrightarrow> VIO \<sigma> v j \<phi> \<Longrightarrow>
-            (\<And>k. k \<in> {j .. (LTP_p \<sigma> i I)} \<Longrightarrow> VIO \<sigma> v k \<psi>) \<Longrightarrow> VIO \<sigma> v i (Extended_MFOTL.Since \<phi> I \<psi>)"
-| VSince_never: "j = (case right I of \<infinity> \<Rightarrow> 0 
-                      | enat b \<Rightarrow> ETP \<sigma> ((\<tau> \<sigma> i) - b)) \<Longrightarrow>
-                   (\<tau> \<sigma> i) \<ge> (\<tau> \<sigma> 0) + left I \<Longrightarrow> 
-                   (\<And>k. k \<in> {j .. (LTP \<sigma> ((\<tau> \<sigma> i) - left I))} \<Longrightarrow> VIO \<sigma> v k \<psi>) \<Longrightarrow> VIO \<sigma> v i (Extended_MFOTL.Since \<phi> I \<psi>)"
-| SUntil: "j \<ge> i \<Longrightarrow> mem (\<tau> \<sigma> j - \<tau> \<sigma> i) I  \<Longrightarrow> SAT \<sigma> v j \<psi> \<Longrightarrow> (\<And>k. k \<in> {i ..< j} \<Longrightarrow> SAT \<sigma> v k \<phi>)
-             \<Longrightarrow> SAT \<sigma> v i (Extended_MFOTL.Until \<phi> I \<psi>)"
+           j \<le> i \<Longrightarrow> (\<tau> \<sigma> 0) + left I \<le> (\<tau> \<sigma> i) \<Longrightarrow> VIO \<sigma> v j \<phi> \<Longrightarrow>
+           (\<And>k. k \<in> {j .. (LTP_p \<sigma> i I)} \<Longrightarrow> VIO \<sigma> v k \<psi>) \<Longrightarrow> VIO \<sigma> v i (MFOTL.Since \<phi> I \<psi>)"
+| VSinceInf: "j = (case right I of \<infinity> \<Rightarrow> 0 
+                      | enat b \<Rightarrow> ETP_p \<sigma> i b) \<Longrightarrow>
+                 (\<tau> \<sigma> i) \<ge> (\<tau> \<sigma> 0) + left I \<Longrightarrow> 
+                 (\<And>k. k \<in> {j .. LTP_p \<sigma> i I} \<Longrightarrow> VIO \<sigma> v k \<psi>) \<Longrightarrow> VIO \<sigma> v i (MFOTL.Since \<phi> I \<psi>)"
+| SUntil: "j \<ge> i \<Longrightarrow> mem (\<delta> \<sigma> j i) I  \<Longrightarrow> SAT \<sigma> v j \<psi> \<Longrightarrow> (\<And>k. k \<in> {i ..< j} \<Longrightarrow> SAT \<sigma> v k \<phi>) \<Longrightarrow> 
+           SAT \<sigma> v i (MFOTL.Until \<phi> I \<psi>)"
 | VUntil: "(case right I of \<infinity> \<Rightarrow> True 
-            | enat b \<Rightarrow> j \<le> LTP \<sigma> ((\<tau> \<sigma> i) + b)) \<Longrightarrow> 
-             j \<ge> i \<Longrightarrow> VIO \<sigma> v j \<phi> \<Longrightarrow> (\<And>k. k \<in> {ETP_f \<sigma> i I .. j} \<Longrightarrow> VIO \<sigma> v k \<psi>) \<Longrightarrow> VIO \<sigma> v i (Extended_MFOTL.Until \<phi> I \<psi>)"
-| VUntil_never: "(\<And>k. k \<in> (case right I of \<infinity> \<Rightarrow> {ETP_f \<sigma> i I ..} 
-                            | enat b \<Rightarrow> {ETP_f \<sigma> i I .. LTP \<sigma> ((\<tau> \<sigma> i) + b)}) \<Longrightarrow> VIO \<sigma> v k \<psi>) \<Longrightarrow>
-                  VIO \<sigma> v i (Extended_MFOTL.Until \<phi> I \<psi>)"
+            | enat b \<Rightarrow> j \<le> LTP_f \<sigma> i b) \<Longrightarrow> 
+           j \<ge> i \<Longrightarrow> VIO \<sigma> v j \<phi> \<Longrightarrow> (\<And>k. k \<in> {ETP_f \<sigma> i I .. j} \<Longrightarrow> VIO \<sigma> v k \<psi>) \<Longrightarrow> 
+           VIO \<sigma> v i (MFOTL.Until \<phi> I \<psi>)"
+| VUntilInf: "(\<And>k. k \<in> (case right I of \<infinity> \<Rightarrow> {ETP_f \<sigma> i I ..} 
+                            | enat b \<Rightarrow> {ETP_f \<sigma> i I .. LTP_f \<sigma> i b}) \<Longrightarrow> VIO \<sigma> v k \<psi>) \<Longrightarrow>
+              VIO \<sigma> v i (MFOTL.Until \<phi> I \<psi>)"
 
-lemma soundness: "(SAT \<sigma> v i \<phi> \<longrightarrow> Extended_MFOTL.sat \<sigma> v i \<phi>) \<and> (VIO \<sigma> v i \<phi> \<longrightarrow> \<not> Extended_MFOTL.sat \<sigma> v i \<phi>)"
+lemma soundness: "(SAT \<sigma> v i \<phi> \<longrightarrow> MFOTL.sat \<sigma> v i \<phi>) \<and> (VIO \<sigma> v i \<phi> \<longrightarrow> \<not> MFOTL.sat \<sigma> v i \<phi>)"
   oops
 
-lemma completeness: "(Extended_MFOTL.sat \<sigma> v i \<phi> \<longrightarrow> SAT \<sigma> v i \<phi>) \<and> (\<not> Extended_MFOTL.sat \<sigma> v i \<phi> \<longrightarrow> VIO \<sigma> v i \<phi>)"
+lemma completeness: "(MFOTL.sat \<sigma> v i \<phi> \<longrightarrow> SAT \<sigma> v i \<phi>) \<and> (\<not> MFOTL.sat \<sigma> v i \<phi> \<longrightarrow> VIO \<sigma> v i \<phi>)"
   oops
 
 end
